<?xml version="1.0" encoding="UTF-8"?>
<rdf:RDF xmlns:rdf="http://www.w3.org/1999/02/22-rdf-syntax-ns#"
     xmlns:rdfs="http://www.w3.org/2000/01/rdf-schema#"
     xmlns:skos="http://www.w3.org/2004/02/skos/core#"
     xmlns:dc="http://purl.org/dc/elements/1.1/" xmlns:dcterms="http://purl.org/dc/terms/"
     xml:base="http://www.language-archives.org/vocabulary/discourse">
     <skos:ConceptScheme rdf:about="http://www.language-archives.org/vocabulary/discourse">
          <dc:title>OLAC Discourse Type Vocabulary</dc:title>
          <dcterms:issued>2012-02-04</dcterms:issued>
          <dc:publisher>Open Language Archives Community</dc:publisher>
          <dc:description>This document specifies the codes, or controlled
               vocabulary, for the Discourse Type extension of the
               Type metadata element. These codes describe the content
               of a resource as structured in such a way as to
               represent a particular type of
               discourse.</dc:description>
          <rdfs:isDefinedBy
               rdf:resource="http://www.language-archives.org/REC/discourse.html"/>
          <rdfs:isDefinedBy
               rdf:resource="http://www.language-archives.org/vocabulary/discourse.rdf"/>
          <skos:hasTopConcept rdf:resource="#dialogue"/>
          <skos:hasTopConcept rdf:resource="#drama"/>
          <skos:hasTopConcept rdf:resource="#formulaic"/>
          <skos:hasTopConcept rdf:resource="#ludic"/>
          <skos:hasTopConcept rdf:resource="#narrative"/>
          <skos:hasTopConcept rdf:resource="#oratory"/>
          <skos:hasTopConcept rdf:resource="#procedural"/>
          <skos:hasTopConcept rdf:resource="#report"/>
          <skos:hasTopConcept rdf:resource="#singing"/>
          <skos:hasTopConcept rdf:resource="#unintelligible_speech"/>
     </skos:ConceptScheme>
     <skos:Concept rdf:about="#dialogue">
          <skos:prefLabel>Dialogue</skos:prefLabel>
          <skos:inScheme
               rdf:resource="http://www.language-archives.org/vocabulary/discourse"/>
          <skos:definition>An interactive discourse with two or more
               participants.</skos:definition>
          <skos:scopeNote/>
          <skos:example>Examples of dialogues include conversations, interviews,
               correspondence, consultations, greetings and
               leave-takings.</skos:example>
     </skos:Concept>
     <skos:Concept rdf:about="#drama">
          <skos:prefLabel>Drama</skos:prefLabel>
          <skos:inScheme
               rdf:resource="http://www.language-archives.org/vocabulary/discourse"/>
          <skos:definition>A planned, creative, rendition of discourse involving
               two or more participants.</skos:definition>
          <skos:scopeNote>Usually a drama involves mimesis of events, either
               real or imagined.</skos:scopeNote>
          <skos:example>Examples of drama include plays, skits, and enacted
               scenes.</skos:example>
     </skos:Concept>
     <skos:Concept rdf:about="#formulaic">
          <skos:prefLabel>Formulaic Discourse</skos:prefLabel>
          <skos:inScheme
               rdf:resource="http://www.language-archives.org/vocabulary/discourse"/>
          <skos:definition>The resource is a ritually or conventionally
               structured discourse.</skos:definition>
          <skos:scopeNote/>
          <skos:example>Examples of formulaic discourse are prayers, curses,
               blessings, charms, curing rituals, marriage vows, and
               oaths.</skos:example>
     </skos:Concept>
     <skos:Concept rdf:about="#ludic">
          <skos:prefLabel>Ludic Discourse</skos:prefLabel>
          <skos:inScheme
               rdf:resource="http://www.language-archives.org/vocabulary/discourse"/>
          <skos:definition>Ludic discourse is language whose primary function is
               to be part of play, or a style of speech that involves
               a creative manipulation of the structures of the
               language. </skos:definition>
          <skos:scopeNote/>
          <skos:example>Examples of ludic discourse are play languages, jokes,
               secret languages, and speech disguises.</skos:example>
     </skos:Concept>
     <skos:Concept rdf:about="#oratory">
          <skos:prefLabel>Oratory</skos:prefLabel>
          <skos:inScheme
               rdf:resource="http://www.language-archives.org/vocabulary/discourse"/>
          <skos:definition>Public speaking, or of speaking eloquently according
               to rules or conventions.</skos:definition>
          <skos:scopeNote/>
          <skos:example>Examples of oratory include sermons, lectures, political
               speeches, and invocations.</skos:example>
     </skos:Concept>
     <skos:Concept rdf:about="#narrative">
          <skos:prefLabel>Narrative Discourse</skos:prefLabel>
          <skos:inScheme
               rdf:resource="http://www.language-archives.org/vocabulary/discourse"/>
          <skos:definition>A monologic discourse which represents temporally
               organized events.</skos:definition>
          <skos:scopeNote/>
          <skos:example>Types of narratives include historical, traditional, and
               personal narratives, myths, folktales, fables, and
               humorous stories.</skos:example>
     </skos:Concept>
     <skos:Concept rdf:about="#procedural">
          <skos:prefLabel>Procedural Discourse</skos:prefLabel>
          <skos:inScheme
               rdf:resource="http://www.language-archives.org/vocabulary/discourse"/>
          <skos:definition>An explanation or description of a method, process,
               or situation having ordered steps. </skos:definition>
          <skos:scopeNote/>
          <skos:example>Examples of procedural discourses include recipes,
               instructions, and plans.</skos:example>
     </skos:Concept>
     <skos:Concept rdf:about="#report">
          <skos:prefLabel>Report</skos:prefLabel>
          <skos:inScheme
               rdf:resource="http://www.language-archives.org/vocabulary/discourse"/>
          <skos:definition>A factual account of some event or
               circumstance.</skos:definition>
          <skos:scopeNote/>
          <skos:example>Examples of reports include news reports, essays, and
               commentaries.</skos:example>
     </skos:Concept>
     <skos:Concept rdf:about="#singing">
          <skos:prefLabel>Singing</skos:prefLabel>
          <skos:inScheme
               rdf:resource="http://www.language-archives.org/vocabulary/discourse"/>
          <skos:definition>"Words or sounds [articulated] in succession with
               musical inflections or modulations of the voice" OED. </skos:definition>
          <skos:scopeNote/>
          <skos:example>Examples of singing include chants, songs, and
               choruses.</skos:example>
     </skos:Concept>
     <skos:Concept rdf:about="#unintelligible_speech">
          <skos:prefLabel>Unintelligible Speech</skos:prefLabel>
          <skos:inScheme
               rdf:resource="http://www.language-archives.org/vocabulary/discourse"/>
          <skos:definition>The resource consists of utterances that are not
               intended to be interpretable as ordinary
               language.</skos:definition>
          <skos:scopeNote/>
          <skos:example>Examples of unintelligible speech include sacred
               languages, Examples of unintelligible speech include
               sacred languages, glossolalia, and singing syllables
               (fa-la-la).</skos:example>
     </skos:Concept>
</rdf:RDF>