<?xml version="1.0" encoding="UTF-8"?>
<rdf:RDF xmlns:rdf="http://www.w3.org/1999/02/22-rdf-syntax-ns#"
	xmlns:rdfs="http://www.w3.org/2000/01/rdf-schema#"
	xmlns:skos="http://www.w3.org/2004/02/skos/core#" xmlns:dc="http://purl.org/dc/elements/1.1/"
	xmlns:dcterms="http://purl.org/dc/terms/"
	xml:base="http://www.language-archives.org/vocabulary/field">
	<skos:ConceptScheme rdf:about="http://www.language-archives.org/vocabulary/field">
		<dc:title>OLAC Linguistic Subject Vocabulary</dc:title>
		<dcterms:issued>2006-04-06</dcterms:issued>
		<dc:publisher>Open Language Archives Community</dc:publisher>
		<dc:description>This document specifies the codes, or suggested vocabulary, for the
			'linguistic' value of the xsi:type attribute of the OLAC Subject element. These codes
			describe the content of a resource as about a particular subfield of linguistic science,
			or about the level of linguistic structure which is the primary concern of a given
			subfield.</dc:description>
		<rdfs:isDefinedBy rdf:resource="http://www.language-archives.org/REC/field.html"/>
		<rdfs:isDefinedBy rdf:resource="http://www.language-archives.org/vocabulary/field.rdf"/>
		<skos:hasTopConcept rdf:resource="#anthropological_linguistics"/>
		<skos:hasTopConcept rdf:resource="#applied_linguistics"/>
		<skos:hasTopConcept rdf:resource="#cognitive_science"/>
		<skos:hasTopConcept rdf:resource="#computational_linguistics"/>
		<skos:hasTopConcept rdf:resource="#discourse_analysis"/>
		<skos:hasTopConcept rdf:resource="#forensic_linguistics"/>
		<skos:hasTopConcept rdf:resource="#general_linguistics"/>
		<skos:hasTopConcept rdf:resource="#historical_linguistics"/>
		<skos:hasTopConcept rdf:resource="#history_of_linguistics"/>
		<skos:hasTopConcept rdf:resource="#language_acquisition"/>
		<skos:hasTopConcept rdf:resource="#language_documentation"/>
		<skos:hasTopConcept rdf:resource="#lexicography"/>
		<skos:hasTopConcept rdf:resource="#linguistic_theories"/>
		<skos:hasTopConcept rdf:resource="#linguistics_and_literature"/>
		<skos:hasTopConcept rdf:resource="#mathematical_linguistics"/>
		<skos:hasTopConcept rdf:resource="#morphology"/>
		<skos:hasTopConcept rdf:resource="#neurolinguistics"/>
		<skos:hasTopConcept rdf:resource="#philosophy_of_language"/>
		<skos:hasTopConcept rdf:resource="#phonetics"/>
		<skos:hasTopConcept rdf:resource="#phonology"/>
		<skos:hasTopConcept rdf:resource="#pragmatics"/>
		<skos:hasTopConcept rdf:resource="#psycholinguistics"/>
		<skos:hasTopConcept rdf:resource="#semantics"/>
		<skos:hasTopConcept rdf:resource="#sociolinguistics"/>
		<skos:hasTopConcept rdf:resource="#syntax"/>
		<skos:hasTopConcept rdf:resource="#text_and_corpus_linguistics"/>
		<skos:hasTopConcept rdf:resource="#translating_and_interpreting"/>
		<skos:hasTopConcept rdf:resource="#typology"/>
		<skos:hasTopConcept rdf:resource="#writing_systems"/>
	</skos:ConceptScheme>
	<skos:Concept rdf:about="#anthropological_linguistics">
		<skos:prefLabel>Anthropological Linguistics</skos:prefLabel>
		<skos:inScheme rdf:resource="http://www.language-archives.org/vocabulary/field"/>
		<skos:definition> The study of language with particular reference to the society and culture
			of the speakers. </skos:definition>
		<skos:scopeNote>Anthropological linguistics often concerns less well-documented languages.
			The definition includes 'ethnolinguistics.' The category is equivalent to the Library of
			Congress subject heading of the same name.</skos:scopeNote>
		<skos:example>The SIL Ethnologue, which collects data on the number on speakers of a
			language and the geographical region in which it is spoken.</skos:example>
	</skos:Concept>
	<skos:Concept rdf:about="#applied_linguistics">
		<skos:prefLabel>Applied Linguistics</skos:prefLabel>
		<skos:inScheme rdf:resource="http://www.language-archives.org/vocabulary/field"/>
		<skos:definition> The use of linguistic methods as applied to language and education, for
			example to literacy or language learning. </skos:definition>
		<skos:scopeNote>The definition includes TESOL, ESL, Second Language Teaching, Second
			Language Learning and Contrastive Linguistics. This category is equivalent to the
			Library of Congress subject heading 'Language and Education,' not the LCSH category
			'Applied Linguistics,' which includes computer applications of linguistics. In the
			'OLAC-Linguistic' extension of the DCMI Subject element, computer applications should be
			classified as Computational Linguistics.</skos:scopeNote>
		<skos:example>Teaching materials, guides for language teachers, and studies of adult
			language learning.</skos:example>
	</skos:Concept>
	<skos:Concept rdf:about="#cognitive_science">
		<skos:prefLabel>Cognitive Science</skos:prefLabel>
		<skos:inScheme rdf:resource="http://www.language-archives.org/vocabulary/field"/>
		<skos:definition> The study of human cognition, particularly as it relates to language. </skos:definition>
		<skos:scopeNote>The category is equivalent to the Library of Congress subject heading of the
			same name.</skos:scopeNote>
		<skos:example>An experiment on language and vision or a book on the study of
			mind.</skos:example>
	</skos:Concept>
	<skos:Concept rdf:about="#computational_linguistics">
		<skos:prefLabel>Computational Linguistics</skos:prefLabel>
		<skos:inScheme rdf:resource="http://www.language-archives.org/vocabulary/field"/>
		<skos:definition> The use of computer science in the study of language. </skos:definition>
		<skos:scopeNote>The definition includes Artificial Intelligence and Natural Language
			Processing, but not Mathematical Linguistics. The category is equivalent to the Library
			of Congress subject heading of the same name.</skos:scopeNote>
		<skos:example>Books and papers dealing with Machine Translation, Text to Speech software,
			and algorithms to parse sentences.</skos:example>
	</skos:Concept>
	<skos:Concept rdf:about="#discourse_analysis">
		<skos:prefLabel>Discourse Analysis</skos:prefLabel>
		<skos:inScheme rdf:resource="http://www.language-archives.org/vocabulary/field"/>
		<skos:definition> The study of the patterns and meanings behind connected speech. </skos:definition>
		<skos:scopeNote>The definition includes Humor Studies, Conversation Analysis, Interactional
			Sociolinguistics, and studies of language use in special circumstances, e.g. Courtroom
			Language. The category is equivalent to the Library of Congress subject heading of the
			same name.</skos:scopeNote>
		<skos:example>Transcripts of discourse, perhaps with turn taking and speaker overlap
			highlighted; papers on Discourse Representation Theory or on different talk types such
			as doctor/patient interaction; and audio and video tapes of interactive discourse which
			might serve as an object of study.</skos:example>
	</skos:Concept>
	<skos:Concept rdf:about="#forensic_linguistics">
		<skos:prefLabel>Forensic Linguistics</skos:prefLabel>
		<skos:inScheme rdf:resource="http://www.language-archives.org/vocabulary/field"/>
		<skos:definition> Applications of linguistic science to the domain of law. </skos:definition>
		<skos:scopeNote>Forensic linguistics refers to the use of linguistic methodology to make
			legal determinations. Analyses of courtroom language are best classified as Discourse
			Analysis. The category is equivalent to the Library of Congress subject heading of the
			same name.</skos:scopeNote>
		<skos:example>Papers on issues in dispute in court cases, e.g., authorship identification,
			assessment of ambiguity in texts, voice attribution.</skos:example>
	</skos:Concept>
	<skos:Concept rdf:about="#general_linguistics">
		<skos:prefLabel>General Linguistics</skos:prefLabel>
		<skos:inScheme rdf:resource="http://www.language-archives.org/vocabulary/field"/>
		<skos:definition> The broad study of linguistics without specialization in any subfield or
			particular reference to a specific linguistic theory. </skos:definition>
		<skos:scopeNote>Resources that cover many subfields in depth, perhaps a dissertation on an
			endangered language with a detailed syntactic and phonological analysis, should be
			classified under all the relevant subfields instead of 'General
			Linguistics'.</skos:scopeNote>
		<skos:example>Broad, often introductory textbooks such as The Cambridge Encyclopaedia of
			Language (Crystal, 1987), and glossaries of linguistic terminology.</skos:example>
	</skos:Concept>
	<skos:Concept rdf:about="#historical_linguistics">
		<skos:prefLabel>Historical Linguistics</skos:prefLabel>
		<skos:inScheme rdf:resource="http://www.language-archives.org/vocabulary/field"/>
		<skos:definition> The diachronic study of language change. </skos:definition>
		<skos:scopeNote>The definition includes Comparative Historical Linguistics, Genetic
			Classification, and philological and etymological study. The last may also be classified
			as Lexicography. The category Historical Linguistics is equivalent to the Library of
			Congress subject heading of the same name.</skos:scopeNote>
		<skos:example>A study of the diachronic development of vowels in Romance.</skos:example>
	</skos:Concept>
	<skos:Concept rdf:about="#history_of_linguistics">
		<skos:prefLabel>History of Linguistics</skos:prefLabel>
		<skos:inScheme rdf:resource="http://www.language-archives.org/vocabulary/field"/>
		<skos:definition> Study of the history and development of linguistic science. </skos:definition>
		<skos:scopeNote/>
		<skos:example>A biography of Ferdinand de Saussure, or an analysis of Plato's discussions on
			language.</skos:example>
	</skos:Concept>
	<skos:Concept rdf:about="#language_acquisition">
		<skos:prefLabel>Language Acquisition</skos:prefLabel>
		<skos:inScheme rdf:resource="http://www.language-archives.org/vocabulary/field"/>
		<skos:definition>The study of the process of acquiring human language.</skos:definition>
		<skos:scopeNote>Language Acquisition may be used to describe materials relating to either
			adult or child language acquisition, and to either first or later language acquisition.
			However, if the materials deal specifically with language teaching, or with the process
			of language learning from a pedagogical point of view, they may be best classified as
			Applied Linguistics. The category is equivalent to the Library of Congress subject
			heading of the same name.</skos:scopeNote>
		<skos:example>Studies of first language acquisition, audio or video tapes of language
			acquisition experiments, and guides to experimental techniques in eliciting acquisition
			data.</skos:example>
	</skos:Concept>
	<skos:Concept rdf:about="#language_documentation">
		<skos:prefLabel>Language Documentation</skos:prefLabel>
		<skos:inScheme rdf:resource="http://www.language-archives.org/vocabulary/field"/>
		<skos:definition> The theory, methodology, and process of language description and
			documentation, including linguistic field methods and fieldwork techniques. </skos:definition>
		<skos:scopeNote/>
		<skos:example>A manual on fieldwork techniques.</skos:example>
	</skos:Concept>
	<skos:Concept rdf:about="#lexicography">
		<skos:prefLabel>Lexicography</skos:prefLabel>
		<skos:inScheme rdf:resource="http://www.language-archives.org/vocabulary/field"/>
		<skos:definition> The process of compiling or studying lexical resources and dictionaries,
			either monolingual or multilingual. </skos:definition>
		<skos:scopeNote>The category is equivalent to the Library of Congress subject heading of the
			same name.</skos:scopeNote>
		<skos:example>Books and papers about creating dictionaries. Swadesh word lists, a bilingual
			Avestan-Engliah dictionary, and a collection of legal terms in a particular
			language.</skos:example>
	</skos:Concept>
	<skos:Concept rdf:about="#linguistics_and_literature">
		<skos:prefLabel>Linguistics and Literature</skos:prefLabel>
		<skos:inScheme rdf:resource="http://www.language-archives.org/vocabulary/field"/>
		<skos:definition>The application of linguistic analysis to literary texts, e.g., fiction,
			drama, or poetry.</skos:definition>
		<skos:scopeNote>The definition includes Stylistics and Poetics. Resources classified under
			this category would also be classified under the Library of Congress subject heading of
			the same name; however, the LCSH does not include Poetics and Stylistics, which are
			separate LCSH fields.</skos:scopeNote>
		<skos:example>An analysis of lexical patterns characteristic of a particular author or
			syntactic constructions used to create specific literary effects.</skos:example>
	</skos:Concept>
	<skos:Concept rdf:about="#linguistic_theories">
		<skos:prefLabel>Linguistic Theories</skos:prefLabel>
		<skos:inScheme rdf:resource="http://www.language-archives.org/vocabulary/field"/>
		<skos:definition>Theories (argued to be) fundamental to linguistic science, often spanning
			more than one subfield such as phonology and syntax. </skos:definition>
		<skos:scopeNote/>
		<skos:example>Papers arguing for or against Universal Grammar, Transformational Grammar, or
			Montague Grammar.</skos:example>
	</skos:Concept>
	<skos:Concept rdf:about="#mathematical_linguistics">
		<skos:prefLabel>Mathematical Linguistics</skos:prefLabel>
		<skos:inScheme rdf:resource="http://www.language-archives.org/vocabulary/field"/>
		<skos:definition> The field of study which treats the mathematical properties of language. </skos:definition>
		<skos:scopeNote>The category is equivalent to the Library of Congress subject heading of the
			same name.</skos:scopeNote>
		<skos:example>A linguistic paper about the formal properties of grammars.</skos:example>
	</skos:Concept>
	<skos:Concept rdf:about="#morphology">
		<skos:prefLabel>Morphology</skos:prefLabel>
		<skos:inScheme rdf:resource="http://www.language-archives.org/vocabulary/field"/>
		<skos:definition> The study of the structure and constituency of individual words. </skos:definition>
		<skos:scopeNote>A resource consisting primarily of data from a morphologically complex
			language should be classifed as 'Language Description' if the primary purpose is to
			describe the structure of the language in question. Use of the Library of Congress
			Subject Heading "Morphophonemics" is deprecated.</skos:scopeNote>
		<skos:example>A paper on morphological theory, Word Grammar (Hudson).</skos:example>
	</skos:Concept>
	<skos:Concept rdf:about="#neurolinguistics">
		<skos:prefLabel>Neurolinguistics</skos:prefLabel>
		<skos:inScheme rdf:resource="http://www.language-archives.org/vocabulary/field"/>
		<skos:definition> The study of brain structure and the physical representation of language
			in the brain. </skos:definition>
		<skos:scopeNote>The category is equivalent to the Library of Congress subject heading of the
			same name.</skos:scopeNote>
		<skos:example>A study of brain damage with respect to language impairment, a study of the
			neurological development of the brain during first language acquisition. The latter
			should also be classified as Language Acquisition.</skos:example>
	</skos:Concept>
	<skos:Concept rdf:about="#philosophy_of_language">
		<skos:prefLabel>Philosophy of Language</skos:prefLabel>
		<skos:inScheme rdf:resource="http://www.language-archives.org/vocabulary/field"/>
		<skos:definition>The application of philosophy to language and linguistic
			theory.</skos:definition>
		<skos:scopeNote>The category is equivalent to the Library of Congress subject heading of the
			same name.</skos:scopeNote>
		<skos:example>A paper on the Sapir-Whorf hypothesis, a comparative study of verbal and
			non-verbal thought.</skos:example>
	</skos:Concept>
	<skos:Concept rdf:about="#phonetics">
		<skos:prefLabel>Phonetics</skos:prefLabel>
		<skos:inScheme rdf:resource="http://www.language-archives.org/vocabulary/field"/>
		<skos:definition> The study and classification of the structure, articulation and perception
			of speech sounds. </skos:definition>
		<skos:scopeNote>The definition includes both articulatory phonetics and acoustic phonetics.
			Datasets, lexicons, and graphic representations of experimental results should be
			classified under Phonetics if they have particular relevance to the sounds of the
			language. The category is equivalent to the Library of Congress subject heading of the
			same name.</skos:scopeNote>
		<skos:example>A sound inventory of a language, a study of the variation of articulation of a
			particular sound.</skos:example>
	</skos:Concept>
	<skos:Concept rdf:about="#phonology">
		<skos:prefLabel>Phonology</skos:prefLabel>
		<skos:inScheme rdf:resource="http://www.language-archives.org/vocabulary/field"/>
		<skos:definition> The study of the patterns and principles behind the sound system of a
			language, or languages in general. </skos:definition>
		<skos:scopeNote>The classification is not limited to phonological analyses. Datasets,
			lexicons, and graphic representations of experimental results should be classified under
			Phonology if they have particular relevance to the sound system of the language. Use of
			the Library of Congress subject heading "Morphophonemics" is
			deprecated.</skos:scopeNote>
		<skos:example>Phonological theories applied to a particular language; that is, a study of
			the syllable structure of a language, or the rules behind sound alternations. Also to be
			included under 'Phonology' are phoneme datasets, field notes on the phonology of a
			language, and papers on phonological theories themselves, such as a critique of
			Optimality Theory.</skos:example>
	</skos:Concept>
	<skos:Concept rdf:about="#pragmatics">
		<skos:prefLabel>Pragmatics</skos:prefLabel>
		<skos:inScheme rdf:resource="http://www.language-archives.org/vocabulary/field"/>
		<skos:definition> The study of the use of language in terms of the context in which it is
			spoken. </skos:definition>
		<skos:scopeNote>The definition includes Non-verbal Communication. The category is equivalent
			to the Library of Congress subject heading of the same name.</skos:scopeNote>
		<skos:example>A study of politeness phenomena, honorifics, deixis or speech
			acts.</skos:example>
	</skos:Concept>
	<skos:Concept rdf:about="#psycholinguistics">
		<skos:prefLabel>Psycholinguistics</skos:prefLabel>
		<skos:inScheme rdf:resource="http://www.language-archives.org/vocabulary/field"/>
		<skos:definition> The application of psychology to linguistics, in terms of the
			psychological mechanisms behind language, such as memory and intelligence (Experimental
			Psycholinguistics). </skos:definition>
		<skos:scopeNote>The category is equivalent to the Library of Congress subject heading of the
			same name.</skos:scopeNote>
		<skos:example>A cross-linguistic study of acquisition of a particular syntactic constraint,
			a study of aphasic children's language development.</skos:example>
	</skos:Concept>
	<skos:Concept rdf:about="#semantics">
		<skos:prefLabel>Semantics</skos:prefLabel>
		<skos:inScheme rdf:resource="http://www.language-archives.org/vocabulary/field"/>
		<skos:definition> The study of the meaning of linguistic structures. </skos:definition>
		<skos:scopeNote>The study of meaning in conversation should be classified as Discourse
			Analysis and not Semantics. The Linguistic Field of Semantics includes meaning at the
			word level ('lexical semantics'). The category is equivalent to the Library of Congress
			subject heading of the same name.</skos:scopeNote>
		<skos:example>A paper on a semantic theory, such as Truth Conditional Semantics. A paper on
			color lexemes in a particular language.</skos:example>
	</skos:Concept>
	<skos:Concept rdf:about="#sociolinguistics">
		<skos:prefLabel>Sociolinguistics</skos:prefLabel>
		<skos:inScheme rdf:resource="http://www.language-archives.org/vocabulary/field"/>
		<skos:definition> The study of language in context of the society that speaks it. </skos:definition>
		<skos:scopeNote>Multilingualism, Folklore, Pidgins and Creoles, Dialectology, Language
			Planning, and Gender Studies should all be classified under 'Sociolinguistics'. The
			category is equivalent to the Library of Congress subject heading of the same
			name.</skos:scopeNote>
		<skos:example>A study of language variation according to such factors as the speakers'
			gender, age, and/or social class.</skos:example>
	</skos:Concept>
	<skos:Concept rdf:about="#syntax">
		<skos:prefLabel>Syntax</skos:prefLabel>
		<skos:inScheme rdf:resource="http://www.language-archives.org/vocabulary/field"/>
		<skos:definition> 'The study of grammatical relations between words and other units within a
			sentence' (Concise Oxford Dictionary of Linguistics). To be distinguished from
			morphology, which applies to units smaller than the word. </skos:definition>
		<skos:scopeNote>The category is equivalent to the Library of Congress subject heading of the
			same name.</skos:scopeNote>
		<skos:example>A syntactic description of a language, using a particular syntactic theory. A
			paper using language data to criticize a syntactic theory.</skos:example>
	</skos:Concept>
	<skos:Concept rdf:about="#text_and_corpus_linguistics">
		<skos:prefLabel>Text and Corpus Linguistics</skos:prefLabel>
		<skos:inScheme rdf:resource="http://www.language-archives.org/vocabulary/field"/>
		<skos:definition> The study of the linguistic properties of an extended passage, text, or
			corpus of texts. </skos:definition>
		<skos:scopeNote>The definition includes Semiotics and Genre Analysis, as well as the
			computational analysis of text corpora.</skos:scopeNote>
		<skos:example>A statistical analysis of the British National Corpus, on the use of modal
			verbs in spoken and written English.</skos:example>
	</skos:Concept>
	<skos:Concept rdf:about="#translating_and_interpreting">
		<skos:prefLabel>Translating and Interpreting</skos:prefLabel>
		<skos:inScheme rdf:resource="http://www.language-archives.org/vocabulary/field"/>
		<skos:definition> The study of the act of converting one language into another, either via
			speech or writing. </skos:definition>
		<skos:scopeNote>The definition includes theoretical discussions of the best translation and
			interpreting methods, and practical aids to interpreting languages. The translated text
			itself may be better classified under 'Language Description' if the purpose of the
			translation is to exemplify the structure of a language. The category is equivalent to
			the Library of Congress subject heading of the same name.</skos:scopeNote>
		<skos:example>A study of the relative merits of different levels of translation (that is,
			literal translation, word-for-word translation and so on).</skos:example>
	</skos:Concept>
	<skos:Concept rdf:about="#typology">
		<skos:prefLabel>Typology</skos:prefLabel>
		<skos:inScheme rdf:resource="http://www.language-archives.org/vocabulary/field"/>
		<skos:definition> The study of the similarites and differences between languages, regardless
			of any genetic relation, and the resulting categorization of language into 'types'. </skos:definition>
		<skos:scopeNote>The definition includes the descriptive and comparative study of Universals.
			The category is equivalent to the Library of Congress subject heading of the same
			name.</skos:scopeNote>
		<skos:example>A paper using data from multiple languages as an argument for or against
			Universal Grammar. An analysis of a poorly documented language in terms of Greenberg's
			Universals.</skos:example>
	</skos:Concept>
	<skos:Concept rdf:about="#writing_systems">
		<skos:prefLabel>Writing Systems</skos:prefLabel>
		<skos:inScheme rdf:resource="http://www.language-archives.org/vocabulary/field"/>
		<skos:definition> The visual representation of spoken language on paper or other media, and
			the issues involved in writing and creating a writing system. </skos:definition>
		<skos:scopeNote>Resources dealing with literacy may be classified as Writing Systems or
			Applied Linguistics or both, depending on whether the resource has substantial pedagogic
			content (Applied Linguistics) or includes an analysis of the graphemic system per se
			(Writing Systems). The category is equivalent to the Library of Congress subject heading
			of the same name.</skos:scopeNote>
		<skos:example>A paper examining issues in a linguist's development of a writing system for a
			previously unwritten language. An examination of pictographic writing systems. A book on
			the decipherment of Linear B.</skos:example>
	</skos:Concept>
</rdf:RDF>