<?xml version="1.0" encoding="UTF-8"?>
<rdf:RDF xmlns:rdf="http://www.w3.org/1999/02/22-rdf-syntax-ns#"
    xmlns:rdfs="http://www.w3.org/2000/01/rdf-schema#"
    xmlns:skos="http://www.w3.org/2004/02/skos/core#"
    xmlns:dc="http://purl.org/dc/elements/1.1/" xmlns:dcterms="http://purl.org/dc/terms/"
    xml:base="http://www.language-archives.org/vocabulary/role">
    <skos:ConceptScheme rdf:about="http://www.language-archives.org/vocabulary/role">
        <dc:title>OLAC Role Vocabulary</dc:title>
        <dcterms:issued>2006-04-06</dcterms:issued>
        <dc:publisher>Open Language Archives Community</dc:publisher>
        <dc:description>Role is an attribute of both the Creator and Contributor elements.
            (Please note that Dublin Core now discourages the use of the Creator
            element, recommending that all Role information be associated with
            Contributor elements.) This document specifies the controlled vocabulary of
            the Role attribute used by OLAC. This attribute specifies the functional
            role of the entity named in the creation of a given
            resource.</dc:description>
        <rdfs:isDefinedBy rdf:resource="http://www.language-archives.org/REC/role.html"/>
        <rdfs:isDefinedBy
            rdf:resource="http://www.language-archives.org/vocabulary/role.rdf"/>
        <skos:hasTopConcept rdf:resource="#annotator"/>
        <skos:hasTopConcept rdf:resource="#author"/>
        <skos:hasTopConcept rdf:resource="#compiler"/>
        <skos:hasTopConcept rdf:resource="#consultant"/>
        <skos:hasTopConcept rdf:resource="#data_inputter"/>
        <skos:hasTopConcept rdf:resource="#depositor"/>
        <skos:hasTopConcept rdf:resource="#developer"/>
        <skos:hasTopConcept rdf:resource="#editor"/>
        <skos:hasTopConcept rdf:resource="#illustrator"/>
        <skos:hasTopConcept rdf:resource="#interpreter"/>
        <skos:hasTopConcept rdf:resource="#interviewer"/>
        <skos:hasTopConcept rdf:resource="#participant"/>
        <skos:hasTopConcept rdf:resource="#performer"/>
        <skos:hasTopConcept rdf:resource="#photographer"/>
        <skos:hasTopConcept rdf:resource="#recorder"/>
        <skos:hasTopConcept rdf:resource="#research_participant"/>
        <skos:hasTopConcept rdf:resource="#researcher"/>
        <skos:hasTopConcept rdf:resource="#responder"/>
        <skos:hasTopConcept rdf:resource="#signer"/>
        <skos:hasTopConcept rdf:resource="#singer"/>
        <skos:hasTopConcept rdf:resource="#speaker"/>
        <skos:hasTopConcept rdf:resource="#sponsor"/>
        <skos:hasTopConcept rdf:resource="#transcriber"/>
        <skos:hasTopConcept rdf:resource="#translator"/>
    </skos:ConceptScheme>
    <skos:Concept rdf:about="#annotator">
        <skos:prefLabel>Annotator</skos:prefLabel>
        <skos:inScheme rdf:resource="http://www.language-archives.org/vocabulary/role"/>
        <skos:definition>The participant produced an annotation of this or a related
            resource.</skos:definition>
        <skos:scopeNote/>
        <skos:example/>
    </skos:Concept>
    <skos:Concept rdf:about="#author">
        <skos:prefLabel>Author</skos:prefLabel>
        <skos:inScheme rdf:resource="http://www.language-archives.org/vocabulary/role"/>
        <skos:definition>The participant contributed original writings to the
            resource.</skos:definition>
        <skos:scopeNote/>
        <skos:example/>
    </skos:Concept>
    <skos:Concept rdf:about="#compiler">
        <skos:prefLabel>Compiler</skos:prefLabel>
        <skos:inScheme rdf:resource="http://www.language-archives.org/vocabulary/role"/>
        <skos:definition>The participant is responsible for collecting the sub-parts of the
            resource together.</skos:definition>
        <skos:scopeNote>This refers to someone who creates a single resource with multiple
            parts, such as a book of short stories, or a person who produces a corpus of
            resources, which may be archived separately.</skos:scopeNote>
        <skos:example>A compiler of a book of short stories or a CD with several songs on
            it; a collector of a corpus of recordings in some language or on a given
            topic; a person who assembles a suite of software tools.</skos:example>
    </skos:Concept>
    <skos:Concept rdf:about="#consultant">
        <skos:prefLabel>Consultant</skos:prefLabel>
        <skos:inScheme rdf:resource="http://www.language-archives.org/vocabulary/role"/>
        <skos:definition>The participant contributes expertise to the creation of a
            work.</skos:definition>
        <skos:scopeNote>This term is commonly used by field linguists for the native
            speakers who work with them in describing and analyzing a language. They
            contribute their expertise in their native language to the resource,
            although their speech, sign, or writing may not appear directly in the
            resource. In some parts of the world the preferred term for this role is
            "informant".</skos:scopeNote>
        <skos:example/>
    </skos:Concept>
    <skos:Concept rdf:about="#data_inputter">
        <skos:prefLabel>Data Inputter</skos:prefLabel>
        <skos:inScheme rdf:resource="http://www.language-archives.org/vocabulary/role"/>
        <skos:definition>The participant was responsible for entering, re-typing, and/or
            structuring the data contained in the resource.</skos:definition>
        <skos:scopeNote/>
        <skos:example/>
    </skos:Concept>
    <skos:Concept rdf:about="#depositor">
        <skos:prefLabel>Depositor</skos:prefLabel>
        <skos:inScheme rdf:resource="http://www.language-archives.org/vocabulary/role"/>
        <skos:definition>The participant was responsible for depositing the resource in an
            archive.</skos:definition>
        <skos:scopeNote/>
        <skos:example/>
    </skos:Concept>
    <skos:Concept rdf:about="#developer">
        <skos:prefLabel>Developer</skos:prefLabel>
        <skos:inScheme rdf:resource="http://www.language-archives.org/vocabulary/role"/>
        <skos:definition>The participant developed the methodology or tools that constitute
            the resource, or that were used to create the resource.</skos:definition>
        <skos:scopeNote/>
        <skos:example>A software programmer, designer, or analyst; a designer of a
            questionnaire or research task.</skos:example>
    </skos:Concept>
    <skos:Concept rdf:about="#editor">
        <skos:prefLabel>Editor</skos:prefLabel>
        <skos:inScheme rdf:resource="http://www.language-archives.org/vocabulary/role"/>
        <skos:definition>The participant reviewed, corrected, and/or tested the
            resource.</skos:definition>
        <skos:scopeNote>This role includes anyone whose role was editorial in nature, such
            as proof-readers, debuggers, testers, etc. It may overlap the Compiler role
            in some cases.</skos:scopeNote>
        <skos:example/>
    </skos:Concept>
    <skos:Concept rdf:about="#illustrator">
        <skos:prefLabel>Illustrator</skos:prefLabel>
        <skos:inScheme rdf:resource="http://www.language-archives.org/vocabulary/role"/>
        <skos:definition>The participant contributed drawings or other illustrations to the
            resource.</skos:definition>
        <skos:scopeNote/>
        <skos:example/>
    </skos:Concept>
    <skos:Concept rdf:about="#interpreter">
        <skos:prefLabel>Interpreter</skos:prefLabel>
        <skos:inScheme rdf:resource="http://www.language-archives.org/vocabulary/role"/>
        <skos:definition>The participant translates in real-time or explains the discourse
            recorded in the resource.</skos:definition>
        <skos:scopeNote>The choice between 'interpreter' and 'translator' may depend on the
            dynamics of the resource creation event or process. Generally, if the
            participant is translating 'live'; that is, while the speaker or signer is
            speaking or signing, she or he should be identified as an interpreter. Also,
            some discourse genres include a participant who interprets or explains a
            performance of some kind.</skos:scopeNote>
        <skos:example>A person translating from English to ASL during a speech; a Kuna chief
            who interprets a chant that another chief has just performed, thus
            completing the ceremony.</skos:example>
    </skos:Concept>
    <skos:Concept rdf:about="#interviewer">
        <skos:prefLabel>Interviewer</skos:prefLabel>
        <skos:inScheme rdf:resource="http://www.language-archives.org/vocabulary/role"/>
        <skos:definition>The participant conducted an interview that forms part of the
            resource.</skos:definition>
        <skos:scopeNote/>
        <skos:example/>
    </skos:Concept>
    <skos:Concept rdf:about="#participant">
        <skos:prefLabel>Participant</skos:prefLabel>
        <skos:inScheme rdf:resource="http://www.language-archives.org/vocabulary/role"/>
        <skos:definition>The participant was present during the creation of the resource,
            but did not contribute substantially to its content.</skos:definition>
        <skos:scopeNote>This role is intended for minor participants such as audience
            members or other peripherally-involved participants in the event. These
            interlocutors need not have been physically present. They could be
            participants in some form of long-distance communication, such as lurkers in
            an online discussion, or they may have participated in general sense of
            having allowed the creation event to take place, such as the mayor of an
            indigenous community.</skos:scopeNote>
        <skos:example/>
    </skos:Concept>
    <skos:Concept rdf:about="#performer">
        <skos:prefLabel>Performer</skos:prefLabel>
        <skos:inScheme rdf:resource="http://www.language-archives.org/vocabulary/role"/>
        <skos:definition>The participant performed some portion of a recorded, filmed, or
            transcribed resource.</skos:definition>
        <skos:scopeNote>It is recommended that this term be used only for creative
            participants whose role is not better indicated by a more specific term,
            such as 'speaker', 'signer', or 'singer'.</skos:scopeNote>
        <skos:example>A person performing a ceremony or delivering an oration or a sermon;
            native speakers re-enacting a traditional genre of speech, such as ritual
            greetings or insults; an actor or musician.</skos:example>
    </skos:Concept>
    <skos:Concept rdf:about="#photographer">
        <skos:prefLabel>Photographer</skos:prefLabel>
        <skos:inScheme rdf:resource="http://www.language-archives.org/vocabulary/role"/>
        <skos:definition>The participant took the photograph, or shot the film, that appears
            in or constitutes the resource.</skos:definition>
        <skos:scopeNote/>
        <skos:example/>
    </skos:Concept>
    <skos:Concept rdf:about="#recorder">
        <skos:prefLabel>Recorder</skos:prefLabel>
        <skos:inScheme rdf:resource="http://www.language-archives.org/vocabulary/role"/>
        <skos:definition>The participant operated the recording machinery used to create the
            resource.</skos:definition>
        <skos:scopeNote/>
        <skos:example/>
    </skos:Concept>
    <skos:Concept rdf:about="#researcher">
        <skos:prefLabel>Researcher</skos:prefLabel>
        <skos:inScheme rdf:resource="http://www.language-archives.org/vocabulary/role"/>
        <skos:definition>The resource was created as part of the participant's research, or
            the research presents interim or final results from the participant's
            research.</skos:definition>
        <skos:scopeNote/>
        <skos:example/>
    </skos:Concept>
    <skos:Concept rdf:about="#research_participant">
        <skos:prefLabel>Research Participant</skos:prefLabel>
        <skos:inScheme rdf:resource="http://www.language-archives.org/vocabulary/role"/>
        <skos:definition>The participant acted as a research subject or responded to a
            questionnaire, the results of which study form the basis of the
            resource.</skos:definition>
        <skos:scopeNote/>
        <skos:example/>
    </skos:Concept>
    <skos:Concept rdf:about="#responder">
        <skos:prefLabel>Responder</skos:prefLabel>
        <skos:inScheme rdf:resource="http://www.language-archives.org/vocabulary/role"/>
        <skos:definition>The participant was an interlocutor in some sort of discourse
            event. </skos:definition>
        <skos:scopeNote>This person's voice can be heard (or their words can be read) in the
            resource, typically saying the language-appropriate equivalent of "uh-huh",
            "amen", "you don't say", etc. This role is sometimes referred to as a
            "yes-sayer", "backchanneler, or "co-conversant".</skos:scopeNote>
        <skos:example/>
    </skos:Concept>
    <skos:Concept rdf:about="#signer">
        <skos:prefLabel>Signer</skos:prefLabel>
        <skos:inScheme rdf:resource="http://www.language-archives.org/vocabulary/role"/>
        <skos:definition>The participant was a principal signer in a resource that consists
            of a recording, a film, or a transcription of a recorded
            resource.</skos:definition>
        <skos:scopeNote>Signers are those whose gestures predominate in a recorded or filmed
            resource. (This resource may be a transcription of that
            recording.)</skos:scopeNote>
        <skos:example>Participants in a recorded conversation, elicitation session, or
            informal narration would be termed Signers. Audience members who do not
            participate beyond the occasional backchannel would be termed
            Responders.</skos:example>
    </skos:Concept>
    <skos:Concept rdf:about="#singer">
        <skos:prefLabel>Singer</skos:prefLabel>
        <skos:inScheme rdf:resource="http://www.language-archives.org/vocabulary/role"/>
        <skos:definition>The participant sang, either individually or as part of a group, in
            a resource that consists of a recording, a film, or a transcription of a
            recorded resource. </skos:definition>
        <skos:scopeNote/>
        <skos:example/>
    </skos:Concept>
    <skos:Concept rdf:about="#speaker">
        <skos:prefLabel>Speaker</skos:prefLabel>
        <skos:inScheme rdf:resource="http://www.language-archives.org/vocabulary/role"/>
        <skos:definition>The participant was a principal speaker in a resource that consists
            of a recording, a film, or a transcription of a recorded
            resource.</skos:definition>
        <skos:scopeNote>Speakers are those whose voices predominate in a recorded or filmed
            resource. (This resource may be a transcription of that recording.)
            Examples: Participants in a recorded conversation, elicitation session, or
            informal narration would be termed Speakers. Audience members who do not
            participate beyond the occasional backchannel would be termed
            Responders.</skos:scopeNote>
        <skos:example/>
    </skos:Concept>
    <skos:Concept rdf:about="#sponsor">
        <skos:prefLabel>Sponsor</skos:prefLabel>
        <skos:inScheme rdf:resource="http://www.language-archives.org/vocabulary/role"/>
        <skos:definition>The participant contributed financial support to the creation of
            the resource.</skos:definition>
        <skos:scopeNote/>
        <skos:example/>
    </skos:Concept>
    <skos:Concept rdf:about="#transcriber">
        <skos:prefLabel>Transcriber</skos:prefLabel>
        <skos:inScheme rdf:resource="http://www.language-archives.org/vocabulary/role"/>
        <skos:definition>The participant produced a transcription of this or a related
            resource.</skos:definition>
        <skos:scopeNote/>
        <skos:example/>
    </skos:Concept>
    <skos:Concept rdf:about="#translator">
        <skos:prefLabel>Translator</skos:prefLabel>
        <skos:inScheme rdf:resource="http://www.language-archives.org/vocabulary/role"/>
        <skos:definition>The participant produced a translation of this or a related
            resource.</skos:definition>
        <skos:scopeNote/>
        <skos:example/>
    </skos:Concept>
</rdf:RDF>