<?xml version="1.0" encoding="UTF-8"?>
<rdf:RDF xmlns:rdf="http://www.w3.org/1999/02/22-rdf-syntax-ns#"
    xmlns:rdfs="http://www.w3.org/2000/01/rdf-schema#"
    xmlns:skos="http://www.w3.org/2004/02/skos/core#" xmlns:dc="http://purl.org/dc/elements/1.1/"
    xmlns:dcterms="http://purl.org/dc/terms/"
    xml:base="http://www.language-archives.org/vocabulary/type">
    <skos:ConceptScheme rdf:about="http://www.language-archives.org/vocabulary/type">
        <dc:title>OLAC Linguistic Data Type Vocabulary</dc:title>
        <dcterms:issued>2006-04-06</dcterms:issued>
        <dc:publisher>Open Language Archives Community</dc:publisher>
        <dc:description>This document specifies the codes, or controlled vocabulary, for the
            Linguistic Data Type extension of the DCMI Type element. These codes describe the
            content of a resource from the standpoint of recognized structural types of linguistic
            information.</dc:description>
        <rdfs:isDefinedBy rdf:resource="http://www.language-archives.org/REC/type.html"/>
        <rdfs:isDefinedBy rdf:resource="http://www.language-archives.org/vocabulary/type.rdf"/>
        <skos:hasTopConcept rdf:resource="#language_description"/>
        <skos:hasTopConcept rdf:resource="#lexicon"/>
        <skos:hasTopConcept rdf:resource="#primary_text"/>
    </skos:ConceptScheme>
    <skos:Concept rdf:about="#lexicon">
        <skos:prefLabel>Lexicon</skos:prefLabel>
        <skos:inScheme rdf:resource="http://www.language-archives.org/vocabulary/type"/>
        <skos:definition>The resource includes a systematic listing of lexical
            items.</skos:definition>
        <skos:scopeNote>Lexicon may be used to describe any resource which includes a systematic
            listing of lexical items. Each lexical item may, but need not, be accompanied by a
            definition, a description of the referent (in the case of proper names), or an
            indication of the item's semantic relationship to other lexical items.</skos:scopeNote>
        <skos:example>Examples include word lists (including comparative word lists), thesauri,
            wordnets, framenets, and dictionaries, including specialized dictionaries such as
            bilingual and multilingual dictionaries, dictionaries of terminology, and dictionaries
            of proper names. Non-word-based examples include phrasal lexicons and lexicons of
            intonational tunes.</skos:example>
    </skos:Concept>
    <skos:Concept rdf:about="#primary_text">
        <skos:prefLabel>Primary Text</skos:prefLabel>
        <skos:inScheme rdf:resource="http://www.language-archives.org/vocabulary/type"/>
        <skos:definition>Linguistic material which is itself the object of study, typically material
            in the subject language which is a performance of a speech event, or the written analog
            of such an event. </skos:definition>
        <skos:scopeNote>Primary Text is used to describe material in the subject language; it
            reflects a speech event, or is the written analog, and embodies linguistic features
            which make it an object of analysis or research. Typically, a primary text has temporal
            structure. Most often in a primary text, the timecourse of some real or fictional
            linguistic event, e.g., a conversation, elicitation session, or imagined scene, is
            carried over into the archived artifact. Note: Primary_text describes the content of the
            resource, not the physical format. A primary text may be recorded in different physical
            media, e.g. as videotaped, audiotaped, or written text. Physical format is described
            using the Format element.</skos:scopeNote>
        <skos:example>Examples of primary texts include transcribed interlinear texts, letters,
            (audiotaped) elicitation sessions, (videotaped) rituals or story-telling sessions, and
            any other recorded speech or writing which exemplifies language structure or use in such
            a way as to become an object of study. When a corpus is a collection of primary texts,
            it should be described both as a primary text (OLAC Linguistic Type) and as a collection
            (DC Type).</skos:example>
    </skos:Concept>
    <skos:Concept rdf:about="#language_description">
        <skos:prefLabel>Language Description</skos:prefLabel>
        <skos:inScheme rdf:resource="http://www.language-archives.org/vocabulary/type"/>
        <skos:definition>The resource describes a language or some aspect(s) of a language via a
            systematic documentation of linguistic structures.</skos:definition>
        <skos:scopeNote>Not every resource commonly termed 'descriptive' should be described with
            this code; for example, a description of Zamenhof, the creator of Esperanto, would not
            be classified using this code. Instead, the code should be reserved for a resource that
            describes a language or some aspect of a language, typically in prose with interspersed
            examples. The similarly named code, Language Documentation (in the Linguistic Subject
            extension) refers to a field of study. This category, Language Description, refers to
            recognized structural types of linguistic information, which are the products of the
            field of study, e.g., grammars and field notes.</skos:scopeNote>
        <skos:example>Examples of descriptions include a formal grammar, a sketch grammar, field
            notes, a phonological sketch.</skos:example>
    </skos:Concept>
</rdf:RDF>